\chapter{Exponentiation of SE(3) Elements}
\label{ch:appendix:math}

The following theorem was found to be very usefull when implementing the kinematics
of a general \gls{aiauv}. Although the proof is simple, and has probably been
derived many times, it is left here for reference.

\begin{theorem}
Let
\begin{subequations}
\begin{align*}
\bm{\omega} &= \begin{bmatrix}\omega_1 & \omega_2 & \omega_3 \end{bmatrix}^T,
\bm{v} = \begin{bmatrix}v_1 & v_2 & v_3 \end{bmatrix}^T \in \R^3 \\
\bm{k} &= \begin{bmatrix}\bm{v}^T & \bm{\omega}^T\end{bmatrix}^T \in \R^6.
\end{align*}
\end{subequations}
Suppose \(\bm{\omega} \neq \bm{0}\), then
\begin{subequations}
\label{eq:app:math:proof1}
\begin{align}
    \exp{\left([\bm{k}]_{\wedge}\right)} &= 
    \exp{\left(\begin{bmatrix}
        0 & -\omega_3 & \omega_2 & v_1 \\
        \omega_3 & 0 & -\omega_1 & v_2 \\
        -\omega_2 & \omega_1 & 0 & v_3 \\
        0 & 0 & 0 & 0
    \end{bmatrix} \right)} = \begin{bmatrix}
        \bm{R} & \bm{V}\bm{v} \\
        \bm{0} & 1
    \end{bmatrix}
\end{align}
\end{subequations}
where
\begin{subequations}
\begin{align*}
    \bm{R} &= \I
    + \frac{\sin{||\bm{\omega}||}}{||\bm{\omega}||}[\bm{\omega}]_{\times}
    + \frac{1-\cos{||\bm{\omega}||}}{||\bm{\omega}||^2}
       [\bm{\omega}]_{\times}[\bm{\omega}]_{\times} \\
    \bm{V} &= \I
    + \frac{1-\cos||\bm{\omega}||}{||\bm{\omega}||^2}[\bm{\omega}]_{\times}
    + \frac{||\bm{\omega}||-\sin||\bm{\omega}||}{||\bm{\omega}||^3}[\bm{\omega}]_{\times}[\bm{\omega}]_{\times}
\end{align*}
\end{subequations}
\end{theorem}

\begin{proof}
\begin{subequations}
\begin{align*}
    \exp{[\bm{k}]_{\wedge}} &:= \sum_{n=0}^{\infty} \frac{1}{n!}[\bm{k}]_{\wedge}^n \\
    &= \I + [\bm{k}]_{\wedge} + \frac{1}{2}[\bm{k}]_{\wedge}^2 + \frac{1}{6}[\bm{k}]_{\wedge}^3 + \frac{1}{24}[\bm{k}]_{\wedge}^4 + \cdots \\
    &= \I + \begin{bmatrix}[\bm{\omega}]_{\times} & \bm{v} \\ \bm{0} & 0\end{bmatrix}
       + \frac{1}{2}\begin{bmatrix}[\bm{\omega}]_{\times}^2 & [\bm{\omega}]_{\times}\bm{v} \\ \bm{0} & 0\end{bmatrix}
       + \frac{1}{6}\begin{bmatrix}[\bm{\omega}]_{\times}^3 & [\bm{\omega}]_{\times}^2\bm{v} \\ \bm{0} & 0\end{bmatrix}
       + \cdots\\
       &= \begin{bmatrix}
\sum_{n=0}^{\infty} \frac{1}{n!}[\bm{\omega}]_{\times}^n &
\left(\sum_{n=0}^{\infty} \frac{1}{\left(n+1\right)!}[\bm{\omega}]_{\times}^n \right) \bm{v}\\
\bm{0} & 1 \\
       \end{bmatrix}
\end{align*}
\end{subequations}
\(\implies \exp{[\bm{k}]_{\wedge}}\) can be written in the form of \autoref{eq:app:math:proof1},
where
\begin{subequations}
\begin{align*}
    \bm{R} &= \sum_{n=0}^{\infty} \frac{1}{n!}[\bm{\omega}]_{\times}^n =: \exp{[\bm{\omega}]_{\times}}\\
    \bm{V} &= \sum_{n=0}^{\infty} \frac{1}{\left(n+1\right)!}[\bm{\omega}]_{\times}^n
\end{align*}
\end{subequations}
The closed-form formula for \(\bm{R}\) is well known and can i derived in the following manner
using that \([\bm{\omega}]_{\times}^3 = -||\bm{\omega}||^2[\bm{\omega}]_{\times}\),
\begin{subequations}
\begin{align*}
\bm{R} &= \I + [\bm{\omega}]_{\times} + \frac{1}{2}[\bm{\omega}]_{\times}^2 + \frac{1}{6}[\bm{\omega}]_{\times}^3 + \frac{1}{24}[\bm{\omega}]_{\times}^4 + \frac{1}{120}[\bm{\omega}]_{\times}^5 + \cdots \\
       &= \I + [\bm{\omega}]_{\times} + \frac{1}{2}[\bm{\omega}]_{\times}^2 -\frac{||\bm{\omega}||^2}{6}[\bm{\omega}]_{\times} - \frac{||\bm{\omega}||^2}{24}[\bm{\omega}]_{\times}^2 + \frac{||\bm{\omega}||^4}{120}[\bm{\omega}]_{\times} + \cdots \\
       &= \I + [\bm{\omega}]_{\times}\left(\frac{1}{1!} - \frac{||\bm{\omega}||^2}{3!} + \frac{||\bm{\omega}||^4}{5!} \cdots\right)
       + [\bm{\omega}]_{\times}^2\left(\frac{1}{2!} - \frac{||\bm{\omega}||^2}{4!} + \frac{||\bm{\omega}||^4}{6!} \cdots\right)\\
       &= \I + \frac{[\bm{\omega}]_{\times}}{||\bm{\omega}||}\sum_{n=0}^{\infty}\frac{(-1)^{n}||\bm{\omega}||^{2n+1}}{(2n+1)!}
       + \frac{[\bm{\omega}]_{\times}^2}{||\bm{\omega}||^2}\sum_{n=1}^{\infty}\frac{(-1)^{n+1}||\bm{\omega}||^{2n}}{2n!} \\
    &= \I
    + \frac{\sin{||\bm{\omega}||}}{||\bm{\omega}||}[\bm{\omega}]_{\times}
    + \frac{1-\cos{||\bm{\omega}||}}{||\bm{\omega}||^2}
       [\bm{\omega}]_{\times}[\bm{\omega}]_{\times}
\end{align*}
\end{subequations} 
The formula for \(\bm{V}\) can be derived in a similar manner:
\begin{subequations}
\begin{align*}
\bm{V} &= \I + \frac{1}{2}\cross{\bm{\omega}}+ \frac{1}{3!}\cross{\bm{\omega}}^2 + \frac{1}{4!}\cross{\bm{\omega}}^3 + \frac{1}{4!}\cross{\bm{\omega}}^4 + \frac{1}{5!}\cross{\bm{\omega}}^5 + \cdots \\
    &= \I + \frac{1}{2}\cross{\bm{\omega}}+ \frac{1}{3!}\cross{\bm{\omega}}^2 - \frac{||\bm{\omega}||^2}{4!}\cross{\bm{\omega}} - \frac{||\bm{\omega}||^2}{5!}\cross{\bm{\omega}}^2 + \frac{||\bm{\omega}||^4}{6!}\cross{\bm{\omega}} \cdots \\
    &= \I + \cross{\bm{\omega}}\left(\frac{1}{2!} - \frac{||\bm{\omega}||^2}{4!} + \frac{||\bm{\omega}||^4}{6!} \cdots\right)
+ \cross{\bm{\omega}}^2\left(\frac{1}{3!} - \frac{||\bm{\omega}||^2}{5!} + \frac{||\bm{\omega}||^4}{7!}\cdots\right)\\
    &= \I + \frac{\cross{\bm{\omega}}}{||\bm{\omega}||^2}\left(\frac{||\bm{\omega}||^2}{2!} - \frac{||\bm{\omega}||^4}{4!} + \frac{||\bm{\omega}||^6}{6!} \cdots\right)
+ \frac{\cross{\bm{\omega}}^2}{||\bm{\omega}||^3}\left(\frac{||\bm{\omega}||^3}{3!} - \frac{||\bm{\omega}||^5}{5!} + \frac{||\bm{\omega}||^7}{7!}\cdots\right) \\
    &= \I + \frac{\cross{\bm{\omega}}}{||\bm{\omega}||^2}\left(1 - \cos{||\bm{\omega}||}\right)
    + \frac{\cross{\bm{\omega}}^2}{||\bm{\omega}||^3}\left(||\bm{\omega}||-\sin{||\bm{\omega}||}\right)
\end{align*}
\end{subequations}
\end{proof}

